pulse/lib/pulse/core/PulseCore.Action.fsti
@@ -200,7 +200,7 @@ val ref_null (#a:Type u#a) (p:pcm a) : ref a p
 val is_ref_null (#a:Type) (#p:FStar.PCM.pcm a) (r:ref a p)
 : b:bool { b <==> r == ref_null p }
 
-val pts_to (#a:Type u#1) (#p:pcm a) (r:ref a p) (v:a) : slprop
+val pts_to (#a:Type u#1) (#p:pcm a) (r:ref a p) (v:a) : vprop
 
 val pts_to_not_null (#a:Type) (#p:FStar.PCM.pcm a) (r:ref a p) (v:a)
 : act (squash (not (is_ref_null r)))
@@ -269,41 +269,78 @@ val gather
     (pts_to r v0 ** pts_to r v1)
     (fun _ -> pts_to r (op pcm v0 v1))
 
-// let property (a:Type)
-//   = a -> prop
+///////////////////////////////////////////////////////////////////
+// Big references
+///////////////////////////////////////////////////////////////////
 
-// val witnessed (#a:Type u#1)
-//               (#pcm:pcm a)
-//               (r:ref a pcm)
-//               (fact:property a)
-//   : Type0
+val big_pts_to (#a:Type u#2) (#p:pcm a) (r:ref a p) (v:a) : slprop
 
-// let stable_property (#a:Type) (pcm:pcm a)
-//   = fact:property a {
-//        FStar.Preorder.stable fact (PP.preorder_of_pcm pcm)
-//     }
+val big_pts_to_not_null (#a:Type) (#p:FStar.PCM.pcm a) (r:ref a p) (v:a)
+: act (squash (not (is_ref_null r)))
+    Ghost
+    emp_inames 
+    (big_pts_to r v)
+    (fun _ -> big_pts_to r v)
 
-// val witness
-//     (#a:Type)
-//     (#pcm:pcm a)
-//     (r:erased (ref a pcm))
-//     (fact:stable_property pcm)
-//     (v:Ghost.erased a)
-//     (pf:squash (forall z. compatible pcm v z ==> fact z))
-// : act (witnessed r fact) UsesInvariants emp_inames (pts_to r v) (fun _ -> pts_to r v)
+val big_alloc
+    (#a:Type)
+    (#pcm:pcm a)
+    (x:a{pcm.refine x})
+: act (ref a pcm)
+      Reifiable
+      emp_inames
+      emp
+      (fun r -> big_pts_to r x)
 
-// val recall
-//     (#a:Type u#1)
-//     (#pcm:pcm a)
-//     (#fact:property a)
-//     (r:erased (ref a pcm))
-//     (v:Ghost.erased a)
-//     (w:witnessed r fact)
-// : act (v1:Ghost.erased a{compatible pcm v v1})
-//     UsesInvariants
-//     emp_inames
-//     (pts_to r v)
-//     (fun v1 -> pts_to r v ** pure (fact v1))
+val big_read
+    (#a:Type)
+    (#p:pcm a)
+    (r:ref a p)
+    (x:erased a)
+    (f:(v:a{compatible p x v}
+        -> GTot (y:a{compatible p y v /\
+                     FStar.PCM.frame_compatible p x v y})))
+: act (v:a{compatible p x v /\ p.refine v})
+      Reifiable
+      emp_inames
+      (big_pts_to r x)
+      (fun v -> big_pts_to r (f v))
+
+val big_write
+    (#a:Type)
+    (#p:pcm a)
+    (r:ref a p)
+    (x y:Ghost.erased a)
+    (f:FStar.PCM.frame_preserving_upd p x y)
+: act unit
+    Reifiable
+    emp_inames
+    (big_pts_to r x)
+    (fun _ -> big_pts_to r y)
+
+val big_share
+    (#a:Type)
+    (#pcm:pcm a)
+    (r:ref a pcm)
+    (v0:FStar.Ghost.erased a)
+    (v1:FStar.Ghost.erased a{composable pcm v0 v1})
+: act unit
+    Ghost
+    emp_inames
+    (big_pts_to r (v0 `op pcm` v1))
+    (fun _ -> big_pts_to r v0 ** big_pts_to r v1)
+
+val big_gather
+    (#a:Type)
+    (#pcm:pcm a)
+    (r:ref a pcm)
+    (v0:FStar.Ghost.erased a)
+    (v1:FStar.Ghost.erased a)
+: act (squash (composable pcm v0 v1))
+    Ghost
+    emp_inames
+    (big_pts_to r v0 ** big_pts_to r v1)
+    (fun _ -> big_pts_to r (op pcm v0 v1))
 
 ///////////////////////////////////////////////////////////////////
 // pure
@@ -337,7 +374,7 @@ val drop (p:slprop)
 ////////////////////////////////////////////////////////////////////////
 [@@erasable]
 val ghost_ref (#[@@@unused] a:Type u#a) ([@@@unused] p:pcm a) : Type u#0
-val ghost_pts_to (#a:Type u#1) (#p:pcm a) (r:ghost_ref p) (v:a) : slprop
+val ghost_pts_to (#a:Type u#1) (#p:pcm a) (r:ghost_ref p) (v:a) : vprop
 
 val ghost_alloc
     (#a:Type u#1)
