pulse/lib/pulse/lib/Pulse.Lib.BigReference.fst
@@ -1,0 +1,189 @@
+(*
+   Copyright 2023 Microsoft Research
+
+   Licensed under the Apache License, Version 2.0 (the "License");
+   you may not use this file except in compliance with the License.
+   You may obtain a copy of the License at
+
+       http://www.apache.org/licenses/LICENSE-2.0
+
+   Unless required by applicable law or agreed to in writing, software
+   distributed under the License is distributed on an "AS IS" BASIS,
+   WITHOUT WARRANTIES OR CONDITIONS OF ANY KIND, either express or implied.
+   See the License for the specific language governing permissions and
+   limitations under the License.
+*)
+
+module Pulse.Lib.BigReference
+open Pulse.Lib.Core
+open Pulse.Main
+open FStar.PCM
+open Pulse.Lib.PCM.Fraction
+
+let ref (a:Type u#2) = pcm_ref (pcm_frac #a)
+let pts_to (#a:Type) (r:ref a) (#[T.exact (`full_perm)] p:perm) (n:a)
+= big_pcm_pts_to r (Some (n, p)) ** pure (perm_ok p)
+
+```pulse
+fn alloc' (#a:Type u#2) (x:a)
+requires emp
+returns r:ref a
+ensures pts_to r x
+{
+  full_values_compatible x;
+  let r = Pulse.Lib.Core.big_alloc #_ #(pcm_frac #a) (Some (x, full_perm));
+  fold (pts_to r #full_perm x);
+  r
+}
+```
+let alloc = alloc'
+
+let read_compat (#a:Type u#1) (x:fractional a)
+                (v:fractional a { compatible pcm_frac x v })
+  : GTot (y:fractional a { compatible pcm_frac y v /\
+                           FStar.PCM.frame_compatible pcm_frac x v y })
+  = x
+
+```pulse
+fn read' (#a:Type u#2) (r:ref a) (#n:erased a) (#p:perm)
+requires pts_to r #p n
+returns x:a
+ensures pts_to r #p n ** pure (reveal n == x)
+{
+  unfold pts_to r #p n;
+  with w. assert (big_pcm_pts_to r w);
+  let x = Pulse.Lib.Core.big_read r w (fun _ -> w);
+  assert pure (compatible pcm_frac w x);
+  assert (big_pcm_pts_to r w);
+  fold (pts_to r #p n);
+  fst (Some?.v x)
+}
+```
+let read = read'
+let ( ! ) #a = read #a
+
+```pulse
+fn write (#a:Type u#2) (r:ref a) (x:a) (#n:erased a)
+requires pts_to r #full_perm n
+ensures pts_to r #full_perm x
+{
+  unfold pts_to r #full_perm n;
+  with w. assert (big_pcm_pts_to r w);
+  Pulse.Lib.Core.big_write r _ _ (mk_frame_preserving_upd n x);
+  fold pts_to r #full_perm x;
+}
+```
+let ( := ) #a = write #a
+
+```pulse
+fn free' (#a:Type u#2) (r:ref a) (#n:erased a)
+requires pts_to r #full_perm n
+ensures emp
+{
+  unfold pts_to r #full_perm n;
+  with w. assert (big_pcm_pts_to r w);
+  Pulse.Lib.Core.big_write r _ _ (mk_frame_preserving_upd_none n);
+  Pulse.Lib.Core.drop_ _;
+}
+```
+let free = free'
+   
+```pulse
+ghost
+fn share' #a (r:ref a) (#v:erased a) (#p:perm)
+requires pts_to r #p v
+ensures pts_to r #(half_perm p) v ** pts_to r #(half_perm p) v
+{
+  unfold pts_to r #p v;
+  rewrite big_pcm_pts_to r (Some (reveal v, p))
+      as  big_pcm_pts_to r (Some (reveal v, half_perm p) `op pcm_frac` Some(reveal v, half_perm p));
+  Pulse.Lib.Core.big_share r (Some (reveal v, half_perm p)) _; //writing an underscore for the first arg also causes a crash
+  fold (pts_to r #(half_perm p) v);
+  fold (pts_to r #(half_perm p) v);
+}
+```
+let share = share'
+
+```pulse
+ghost
+fn gather' #a (r:ref a) (#x0 #x1:erased a) (#p0 #p1:perm)
+requires pts_to r #p0 x0 ** pts_to r #p1 x1
+ensures pts_to r #(sum_perm p0 p1) x0 ** pure (x0 == x1)
+{ 
+  unfold pts_to r #p0 x0;
+  unfold pts_to r #p1 x1;
+  Pulse.Lib.Core.big_gather r (Some (reveal x0, p0)) (Some (reveal x1, p1));
+  fold (pts_to r #(sum_perm p0 p1) x0)
+}
+```
+let gather = gather'
+
+let share2 (#a:Type) (r:ref a) (#v:erased a) = share r #v #full_perm
+let gather2 (#a:Type) (r:ref a) (#x0 #x1:erased a) = gather r #x0 #x1 #one_half #one_half
+
+```pulse
+fn free_with_frame #a (r:ref a) (frame:vprop)
+requires frame ** (exists* (x:a). pts_to r x)
+ensures frame
+{
+  free r;
+}
+```
+
+(* this is universe-polymorphic in ret_t; so can't define it in Pulse yet *)
+let with_local
+    (#a:Type u#2)
+    (init:a)
+    (#pre:vprop)
+    (#ret_t:Type u#a)
+    (#post:ret_t -> vprop) 
+    (body: (r:ref a -> stt ret_t (pre ** pts_to r init) (fun v -> post v ** (exists* (x:a). pts_to r x))))
+= let m1
+    : stt (ref a) (emp ** pre) (fun r -> pts_to r init ** pre)
+    = frame_stt pre (alloc init)
+  in
+  let pf_post : vprop_post_equiv (fun r -> pts_to r init ** pre) (fun r -> pre ** pts_to r init)
+    = intro_vprop_post_equiv _ _ (fun r -> vprop_equiv_comm (pts_to r #full_perm init) pre)
+  in
+  let m1 
+    : stt (ref a) pre (fun r -> pre ** pts_to r init)
+    = sub_stt _ _ (vprop_equiv_unit pre) pf_post m1
+  in
+  let body (r:ref a)
+    : stt ret_t (pre ** pts_to r init) post
+    = bind_stt (body r) (fun v -> bind_stt (free_with_frame #a r (post v)) (fun _ -> return_stt_noeq v post))
+  in
+  bind_stt m1 body
+
+         
+```pulse
+ghost
+fn pts_to_injective_eq'
+    (#a:Type)
+    (#p0 #p1:perm)
+    (#v0 #v1:a)
+    (r:ref a)
+requires pts_to r #p0 v0 ** pts_to r #p1 v1
+ensures pts_to r #p0 v0 ** pts_to r #p1 v1 ** pure (v0 == v1)
+{
+  unfold pts_to r #p0 v0;
+  unfold pts_to r #p1 v1;
+  Pulse.Lib.Core.big_gather r (Some (v0, p0)) (Some (v1, p1));
+  Pulse.Lib.Core.big_share r (Some (v0, p0)) (Some (v1, p1));
+  fold pts_to r #p0 v0;
+  fold pts_to r #p1 v1;
+}
+```
+let pts_to_injective_eq = pts_to_injective_eq'
+
+```pulse
+ghost
+fn pts_to_perm_bound' (#a:_) (#p:_) (r:ref a) (#v:a)
+requires pts_to r #p v
+ensures pts_to r #p v ** pure (p `lesser_equal_perm` full_perm)
+{
+  unfold pts_to r #p v;
+  fold pts_to r #p v;
+}
+```
+let pts_to_perm_bound = pts_to_perm_bound'
